coq/theories/automation/Automation.v
@@ -10,11 +10,27 @@ Require Import Lia Nat Arith.
 
 Definition empty_state : state := init_state lnil [].
 
-
 (* TODO(kπ) figure out a good example, this one gets constant folded *)
 Example arith_example : forall n m,
-  exists prog, Env.empty |- (prog, empty_state) ---> ([Num (let x := 1 in x + n - m)], empty_state).
+  exists prog, Env.empty |- (prog, empty_state) ---> ([Num ((fun x => x + n - m) 1)], empty_state).
 Proof.
   intros.
-  eauto with automation.
+  eexists. (* TODO(kπ) this simplifies my function :/ Is this a problem with normal code?*)
+  eapply auto_let; eauto; intros.
+  repeat match goal with
+  | |- context[_ + _] => eapply auto_num_add; eauto
+  | |- context[_ - _] => eapply auto_num_sub; eauto
+  end.
+  (* TODO(kπ) *)
 Qed.
+
+(*
+TODO(kπ) Problems:
+- in HOL4 (let x = a in b) is encoded as ((fn x => b) a) Do we have to do the
+  same? Add a preprocessing step or sth?
+- in the HOL4 version (AFAIK) only limited matches on datatypes are supported,
+  but the problem is that matches in HOL4 are represented using `CASE functions`
+  e.g.
+  list case [ ] f1 f2 = f1
+  list case (x :: xs) f1 f2 = f2 x xs
+*)
